database/Extract.v
@@ -5,9 +5,10 @@ From Coq Require Extraction.
 From RecoveryRefinement Require Import Helpers.ExtrMachinePrimitives.
 From RecoveryRefinement Require Import Database.ExtrBaseLayer.
 From RecoveryRefinement Require Import Database.ExtractionExamples.
+From RecoveryRefinement Require Import Database.Simple.SimpleDb.
 
 Extraction Language Haskell.
 
-Separate Extraction ExtractionExamples.
+Separate Extraction ExtractionExamples SimpleDb.
 
 Cd "../../..".
