src/Helpers/ExtrMachinePrimitives.v
@@ -8,6 +8,9 @@ From RecoveryRefinement Require Import Helpers.MachinePrimitives.
 Extraction Language Haskell.
 
 Extract Inductive uint64 => "Lib.Word64" ["Prelude.fromIntegral"].
+Extract Constant uint64_from_le => "Lib.uint64_from_le".
+Extract Constant uint64_to_le => "Lib.uint64_to_le".
+
 (* fromNum might be used by constants, but there shouldn't be any use case for
 toNum *)
 Extract Inlined Constant toNum => "undefined".
@@ -20,6 +23,11 @@ Extract Constant compare => "Lib.compare".
 
 Extract Constant byte => "Lib.Word8".
 (* extract these to a real type, but don't provide any constructor *)
-Extract Inductive ByteString => "Lib.ByteString" ["undefined"].
+Extract Inductive ByteString => "Lib.ByteString" ["Lib.byteString_pack"] "Lib.byteString_rec".
+Extract Constant getBytes => "Lib.byteString_unpack".
+Extract Constant BS.toString => "Lib.byteString_to_String".
+Extract Constant BS.fromString => "Lib.string_to_ByteString".
+Extract Constant BS.drop => "Lib.bs_drop".
+Extract Constant BS.take => "Lib.bs_take".
 
 Extract Constant Fd => "Lib.Fd".
